added & grouped theorems

Circuits.v
@@ -1,11 +1,21 @@
 (* Modeling Electrical Circuits
  * CS 6115 Small Project
  * Brittany Nkounkou and Yao Wang
- *
- * 2/24/15: initial circuit and function definitions -BN
  *)
 
+
+
+Require Import Fin Vector.
+Import VectorNotations.
+
+Require Import Plus.
+
+
+
+(* ~~~~~~~ DEFINITIONS ~~~~~~~ *)
+
 Inductive Circuit : nat -> nat -> Type :=
+  | none : Circuit 0 0
   | high : Circuit 0 1
   | low  : Circuit 0 1
   | wire : Circuit 1 1
@@ -23,17 +33,18 @@ Inductive Circuit : nat -> nat -> Type :=
 
 Fixpoint area {i o} (C : Circuit i o) : nat :=
   match C with
+    | none => 0
     | high => 0
     | low  => 0
     | wire => 0
     | inv  => 108
-	| buf  => 144
+    | buf  => 144
     | and  => 216
     | or   => 216
     | xor  => 360
     | nand => 144
-	| nor  => 144
-	| xnor => 396
+    | nor  => 144
+    | xnor => 396
     | and3 => 252
     | comp _ _ _ c1 c2 => (area c1) + (area c2)
     | par _ _ _ _ c1 c2 => (area c1) + (area c2)
@@ -41,24 +52,22 @@ Fixpoint area {i o} (C : Circuit i o) : nat :=
 
 Fixpoint delay {i o} (C : Circuit i o) : nat :=
   match C with
+    | none => 0
     | high => 0
     | low  => 0
     | wire => 0
     | inv  => 23
-	| buf  => 66
+    | buf  => 66
     | and  => 53
     | or   => 62
     | xor  => 88
     | nand => 31
-	| nor  => 50
-	| xnor => 89
+    | nor  => 50
+    | xnor => 89
     | and3 => 68
     | comp _ _ _ c1 c2 => (delay c1) + (delay c2)
     | par _ _ _ _ c1 c2 => max (delay c1) (delay c2)
   end.
-
-Require Import Fin Vector.
-Import VectorNotations.
 
 Definition BoolVect := t bool.
 
@@ -76,50 +85,185 @@ Fixpoint bv_plus_right {n m} (bv : BoolVect (n + m)) : BoolVect m :=
 
 Fixpoint behavior {i o} (C : Circuit i o) : BoolVect i -> BoolVect o :=
   match C with
+    | none => fun _ => []
     | high => fun _ => [true]
     | low  => fun _ => [false]
     | wire => fun bv => bv
     | inv  => fun bv => map negb bv
-	| buf  => fun bv => bv
+    | buf  => fun bv => bv
     | and  => fun bv => [fold_right andb bv true]
     | or   => fun bv => [fold_right orb bv false]
     | xor  => fun bv => [xorb bv[@ F1] bv[@ FS F1]]
     | nand => fun bv => [negb (fold_right andb bv true)]
-	| nor  => fun bv => [negb (fold_right orb bv false)]
-	| xnor => fun bv => [negb (xorb bv[@ F1] bv[@ FS F1])]
+    | nor  => fun bv => [negb (fold_right orb bv false)]
+    | xnor => fun bv => [negb (xorb bv[@ F1] bv[@ FS F1])]
     | and3 => fun bv => [fold_right andb bv true]
     | comp _ _ _ c1 c2 => fun bv => behavior c2 (behavior c1 bv)
     | par _ _ _ _ c1 c2 => fun bv => append (behavior c1 (bv_plus_left bv))
                                             (behavior c2 (bv_plus_right bv))
   end.
 
-Theorem area_comp: forall (m n : nat) (A : Circuit m n) (B : Circuit n m),
+
+
+(* ~~~~~~~ ASSOCIATIVITY ~~~~~~~ *)
+
+Theorem area_comp_assoc : forall (m n o p : nat) (A : Circuit m n) (B : Circuit n o) (C : Circuit o p),
+  area (comp A (comp B C)) = area (comp (comp A B) C).
+Proof. Admitted.
+
+Theorem area_par_assoc : forall (m n o p q r : nat) (A : Circuit m n) (B : Circuit o p) (C : Circuit q r),
+  area (par A (par B C)) = area (par (par A B) C).
+Proof. Admitted.
+
+Theorem delay_comp_assoc : forall (m n o p : nat) (A : Circuit m n) (B : Circuit n o) (C : Circuit o p),
+  delay (comp A (comp B C)) = delay (comp (comp A B) C).
+Proof. Admitted.
+
+Theorem delay_par_assoc : forall (m n o p q r : nat) (A : Circuit m n) (B : Circuit o p) (C : Circuit q r),
+  delay (par A (par B C)) = delay (par (par A B) C).
+Proof. Admitted.
+
+Theorem behavior_comp_assoc : forall (m n o p : nat) (A : Circuit m n) (B : Circuit n o) (C : Circuit o p),
+  behavior (comp A (comp B C)) = behavior (comp (comp A B) C).
+Proof. Admitted.
+
+Theorem behavior_par_assoc : forall (m n o p q r : nat) (A : Circuit m n) (B : Circuit o p) (C : Circuit q r),
+  behavior (par A (par B C)) = eq_rect_r (fun x => BoolVect x -> _)
+                                         (eq_rect_r (fun x => _ -> BoolVect x)
+                                                    (behavior (par (par A B) C))
+                                                    (plus_assoc _ _ _))
+                                         (plus_assoc _ _ _).
+Proof. Admitted.
+
+
+
+(* ~~~~~~~ IDENTITY ELEMENTS ~~~~~~~ *)
+
+Fixpoint par_wire (n : nat) : Circuit n n :=
+  match n with
+    | O => none
+    | S n' => par wire (par_wire n')
+  end.
+
+Theorem area_comp_ident_l : forall (m n : nat) (A : Circuit m n),
+  area (comp (par_wire m) A) = area A.
+Proof. Admitted.
+
+Theorem area_comp_ident_R : forall (m n : nat) (A : Circuit m n),
+  area (comp A (par_wire n)) = area A.
+Proof. Admitted.
+
+Theorem area_par_ident_l : forall (m n : nat) (A : Circuit m n),
+  area (par none A) = area A.
+Proof. Admitted.
+
+Theorem area_par_ident_R : forall (m n : nat) (A : Circuit m n),
+  area (par A none) = area A.
+Proof. Admitted.
+
+Theorem delay_comp_ident_l : forall (m n : nat) (A : Circuit m n),
+  delay (comp (par_wire m) A) = delay A.
+Proof. Admitted.
+
+Theorem delay_comp_ident_R : forall (m n : nat) (A : Circuit m n),
+  delay (comp A (par_wire n)) = delay A.
+Proof. Admitted.
+
+Theorem delay_par_ident_l : forall (m n : nat) (A : Circuit m n),
+  delay (par none A) = delay A.
+Proof. Admitted.
+
+Theorem delay_par_ident_R : forall (m n : nat) (A : Circuit m n),
+  delay (par A none) = delay A.
+Proof. Admitted.
+
+Theorem behavior_comp_ident_l : forall (m n : nat) (A : Circuit m n),
+  behavior (comp (par_wire m) A) = behavior A.
+Proof. Admitted.
+
+Theorem behavior_comp_ident_R : forall (m n : nat) (A : Circuit m n),
+  behavior (comp A (par_wire n)) = behavior A.
+Proof. Admitted.
+
+Theorem behavior_par_ident_l : forall (m n : nat) (A : Circuit m n),
+  behavior (par none A) = behavior A.
+Proof. Admitted.
+
+Theorem behavior_par_ident_R : forall (m n : nat) (A : Circuit m n),
+  behavior (par A none) = eq_rect_r (fun x => BoolVect x -> _)
+                                    (eq_rect_r (fun x => _ -> BoolVect x)
+                                               (behavior A)
+                                               (plus_0_r _))
+                                    (plus_0_r _).
+Proof. Admitted.
+
+
+
+(* ~~~~~~~ COMMUTATIVITY ~~~~~~~ *)
+
+Theorem area_comp_comm : forall (m n : nat) (A : Circuit m n) (B : Circuit n m),
   area (comp A B) = area (comp B A).
 Proof. Admitted.
 
-Theorem delay_comp: forall (m n : nat) (A : Circuit m n) (B : Circuit n m),
-  delay (comp A B) = delay (comp B A).
-Proof. Admitted.
-
-Theorem area_par: forall (m n : nat) (A : Circuit m n) (B : Circuit n m),
+Theorem area_par_comm : forall (m n o p : nat) (A : Circuit m n) (B : Circuit o p),
   area (par A B) = area (par B A).
 Proof. Admitted.
 
-Theorem delay_par: forall (m n : nat) (A : Circuit m n) (B : Circuit n m),
+Theorem delay_comp_comm : forall (m n : nat) (A : Circuit m n) (B : Circuit n m),
+  delay (comp A B) = delay (comp B A).
+Proof. Admitted.
+
+Theorem delay_par_comm : forall (m n o p : nat) (A : Circuit m n) (B : Circuit o p),
   delay (par A B) = delay (par B A).
 Proof. Admitted.
 
-Theorem comp_par_area: forall (m n o p q r: nat) (A : Circuit m n) (B : Circuit n o) (C : Circuit p q) (D : Circuit q r),
+
+
+(* ~~~~~~~ DISTRIBUTIVITY ~~~~~~~ *)
+
+Theorem delay_distr_l : forall (m n o p q : nat) (A : Circuit m (n + p)) (B : Circuit n o) (C : Circuit p q),
+  delay (comp A (par B C)) = delay (par (comp A (par B (par_wire p))) (comp A (par (par_wire n) C))).
+Proof. Admitted.
+
+Theorem delay_distr_r : forall (m n o p q : nat) (B : Circuit m n) (C : Circuit o p) (A : Circuit (n + p) q),
+  delay (comp (par B C) A) = delay (par (comp (par B (par_wire p)) A) (comp (par (par_wire n) C) A)).
+Proof. Admitted.
+
+
+
+(* ~~~~~~~ IDEMPOTENCE ~~~~~~~ *)
+
+Theorem delay_par_idemp : forall (m n : nat) (A : Circuit m n),
+  delay (par A A) = delay A.
+Proof. Admitted.
+
+
+
+(* ~~~~~~~ I DON'T KNOW WHAT TO CALL THIS. IT'S KIND OF LIKE TRANSPOSITION. MANHATTAN EQUIVALENCE? ~~~~~~~ *)
+(* TODO : generalize the theorems below to account for any finite number of rows/column
+        : area_manhattan, comp_manhattan, behavior_manhattan *)
+
+Theorem area_comp_par : forall (m n o p q r : nat) (A : Circuit m n) (B : Circuit n o) (C : Circuit p q) (D : Circuit q r),
   area (par (comp A B) (comp C D)) = area (comp (par A C) (par B D)).
 Proof. Admitted.
 
-Theorem comp_par_delay: forall (m n o p q r: nat) (A : Circuit m n) (B : Circuit n o) (C : Circuit p q) (D : Circuit q r),
+Theorem delay_comp_par : forall (m n o p q r : nat) (A : Circuit m n) (B : Circuit n o) (C : Circuit p q) (D : Circuit q r),
   delay (par (comp A B) (comp C D)) = delay (comp (par A C) (par B D)).
 Proof. Admitted.
 
-Theorem comp_par: forall (m n o p q r: nat) (A : Circuit m n) (B : Circuit n o) (C : Circuit p q) (D : Circuit q r),
+Theorem behavior_comp_par : forall (m n o p q r : nat) (A : Circuit m n) (B : Circuit n o) (C : Circuit p q) (D : Circuit q r),
   behavior (par (comp A B) (comp C D)) = behavior (comp (par A C) (par B D)).
 Proof. Admitted.
 
-Theorem diff_delay: behavior nand = behavior (comp and inv) \/ area nand <> area (comp and inv).
+
+
+(* ~~~~~~~ FACTS ~~~~~~~ *)
+
+Theorem nand_vs_and_inv : behavior nand = behavior (comp and inv) /\ area nand < area (comp and inv) /\ delay nand < area (comp and inv).
+Proof. Admitted.
+
+Theorem nand_minimal_area : ~ exists (C : Circuit 2 1), behavior C = behavior nand /\ area C < area nand.
+Proof. Admitted.
+
+Theorem nand_minimal_delay : ~ exists (C : Circuit 2 1), behavior C = behavior nand /\ delay C < delay nand.
 Proof. Admitted.
